theories/typing/programs.v
@@ -10,9 +10,8 @@ Section typing.
   (* This is an iProp because it is also used by the function type. *)
   Definition typed_body (E : elctx) (L : llctx) (C : cctx) (T : tctx)
                         (e : expr) : iProp Σ :=
-    (∀ tid qE, lft_ctx -∗ na_own tid ⊤ -∗
-               elctx_interp E qE -∗ llctx_interp L 1 -∗
-               (elctx_interp E qE -∗ cctx_interp tid C) -∗ tctx_interp tid T -∗
+    (∀ tid, lft_ctx -∗ elctx_interp E -∗ na_own tid ⊤ -∗ llctx_interp L 1 -∗
+               cctx_interp tid C -∗ tctx_interp tid T -∗
                WP e {{ _, cont_postcondition }})%I.
   Global Arguments typed_body _%EL _%LL _%CC _%TC _%E.
 
@@ -35,10 +34,10 @@ Section typing.
            (typed_body E L).
   Proof.
     intros C1 C2 HC T1 T2 HT e ? <-. iIntros "H".
-    iIntros (tid qE) "#LFT Htl HE HL HC HT".
-    iMod (HT with "LFT HE HL HT") as "(HE & HL & HT)".
-    iApply ("H" with "LFT Htl HE HL [HC] HT").
-    iIntros "HE". by iApply (HC with "LFT HC").
+    iIntros (tid) "#LFT #HE Htl HL HC HT".
+    iMod (HT with "LFT HE HL HT") as "(HL & HT)".
+    iApply ("H" with "LFT HE Htl HL [HC] HT").
+    by iApply (HC with "LFT HE HC").
   Qed.
 
   Global Instance typed_body_mono_flip E L:
@@ -49,19 +48,19 @@ Section typing.
   (** Instruction *)
   Definition typed_instruction (E : elctx) (L : llctx)
              (T1 : tctx) (e : expr) (T2 : val → tctx) : iProp Σ :=
-    (∀ tid qE, lft_ctx -∗ na_own tid ⊤ -∗
-              elctx_interp E qE -∗ llctx_interp L 1 -∗ tctx_interp tid T1 -∗
-              WP e {{ v, na_own tid ⊤ ∗ elctx_interp E qE ∗
+    (∀ tid, lft_ctx -∗ elctx_interp E -∗ na_own tid ⊤ -∗
+              llctx_interp L 1 -∗ tctx_interp tid T1 -∗
+              WP e {{ v, na_own tid ⊤ ∗
                          llctx_interp L 1 ∗ tctx_interp tid (T2 v) }})%I.
   Global Arguments typed_instruction _%EL _%LL _%TC _%E _%TC.
 
   (** Writing and Reading **)
   Definition typed_write (E : elctx) (L : llctx) (ty1 ty ty2 : type) : iProp Σ :=
-    (□ ∀ v tid F qE qL, ⌜lftE ∪ (↑lrustN) ⊆ F⌝ →
-      lft_ctx -∗ elctx_interp E qE -∗ llctx_interp L qL -∗ ty1.(ty_own) tid [v] ={F}=∗
+    (□ ∀ v tid F qL, ⌜lftE ∪ (↑lrustN) ⊆ F⌝ →
+      lft_ctx -∗ elctx_interp E -∗ llctx_interp L qL -∗ ty1.(ty_own) tid [v] ={F}=∗
         ∃ (l : loc) vl, ⌜length vl = ty.(ty_size) ∧ v = #l⌝ ∗ l ↦∗ vl ∗
           (▷ l ↦∗: ty.(ty_own) tid ={F}=∗
-            elctx_interp E qE ∗ llctx_interp L qL ∗ ty2.(ty_own) tid [v]))%I.
+            llctx_interp L qL ∗ ty2.(ty_own) tid [v]))%I.
   Global Arguments typed_write _%EL _%LL _%T _%T _%T.
 
   (* Technically speaking, we could remvoe the vl quantifiaction here and use
@@ -70,11 +69,11 @@ Section typing.
      that nobody could possibly have changed the vl (because only half the
      fraction was given). So we go with the definition that is easier to prove. *)
   Definition typed_read (E : elctx) (L : llctx) (ty1 ty ty2 : type) : iProp Σ :=
-    (□ ∀ v tid F qE qL, ⌜lftE ∪ (↑lrustN) ⊆ F⌝ →
-      lft_ctx -∗ na_own tid F -∗
-      elctx_interp E qE -∗ llctx_interp L qL -∗ ty1.(ty_own) tid [v] ={F}=∗
+    (□ ∀ v tid F qL, ⌜lftE ∪ (↑lrustN) ⊆ F⌝ →
+      lft_ctx -∗ elctx_interp E -∗ na_own tid F -∗
+      llctx_interp L qL -∗ ty1.(ty_own) tid [v] ={F}=∗
         ∃ (l : loc) vl q, ⌜v = #l⌝ ∗ l ↦∗{q} vl ∗ ▷ ty.(ty_own) tid vl ∗
-              (l ↦∗{q} vl ={F}=∗ na_own tid F ∗ elctx_interp E qE ∗
+              (l ↦∗{q} vl ={F}=∗ na_own tid F ∗
                               llctx_interp L qL ∗ ty2.(ty_own) tid [v]))%I.
   Global Arguments typed_read _%EL _%LL _%T _%T _%T.
 End typing.
@@ -100,13 +99,11 @@ Section typing_rules.
     typed_body ((κ1 ⊑ κ2) :: (κ2 ⊑ κ1) :: E) L C T e →
     typed_body E ((κ1 ⊑ [κ2]%list) :: L) C T e.
   Proof.
-    iIntros (He tid qE) "#LFT Htl HE HL HC HT".
+    iIntros (He tid) "#LFT #HE Htl HL HC HT".
     rewrite /llctx_interp big_sepL_cons. iDestruct "HL" as "[Hκ HL]".
     iMod (lctx_equalize_lft with "LFT Hκ") as "[Hκ1 Hκ2]".
-    iApply (He with "LFT Htl [Hκ1 Hκ2 HE] HL [HC] HT").
-    - rewrite /elctx_interp !big_sepL_cons. by iFrame.
-    - rewrite /elctx_interp !big_sepL_cons. iIntros "(_ & _ & HE)".
-      iApply "HC". done.
+    iApply (He with "LFT [Hκ1 Hκ2 HE] Htl HL HC HT").
+    rewrite /elctx_interp !big_sepL_cons. by iFrame.
   Qed.
 
   Lemma type_let' E L T1 T2 (T : tctx) C xb e e' :
@@ -115,11 +112,11 @@ Section typing_rules.
     (∀ v : val, typed_body E L C (T2 v ++ T) (subst' xb v e')) -∗
     typed_body E L C (T1 ++ T) (let: xb := e in e').
   Proof.
-    iIntros (Hc) "He He'". iIntros (tid qE) "#LFT Htl HE HL HC HT". rewrite tctx_interp_app.
-    iDestruct "HT" as "[HT1 HT]". wp_bind e. iApply (wp_wand with "[He HE HL HT1 Htl]").
-    { iApply ("He" with "LFT Htl HE HL HT1"). }
-    iIntros (v) "/= (Htl & HE & HL & HT2)". iApply wp_let; first wp_done.
-    iModIntro. iApply ("He'" with "LFT Htl HE HL HC [HT2 HT]").
+    iIntros (Hc) "He He'". iIntros (tid) "#LFT #HE Htl HL HC HT". rewrite tctx_interp_app.
+    iDestruct "HT" as "[HT1 HT]". wp_bind e. iApply (wp_wand with "[He HL HT1 Htl]").
+    { iApply ("He" with "LFT HE Htl HL HT1"). }
+    iIntros (v) "/= (Htl & HL & HT2)". iApply wp_let; first wp_done.
+    iModIntro. iApply ("He'" with "LFT HE Htl HL HC [HT2 HT]").
     rewrite tctx_interp_app. by iFrame.
   Qed.
 
@@ -152,10 +149,10 @@ Section typing_rules.
     (∀ κ, typed_body E ((κ ⊑ κs) :: L) C T e) -∗
     typed_body E L C T (Newlft ;; e).
   Proof.
-    iIntros (Hc) "He". iIntros (tid qE) "#LFT Htl HE HL HC HT".
+    iIntros (Hc) "He". iIntros (tid) "#LFT #HE Htl HL HC HT".
     iMod (lft_create with "LFT") as (Λ) "[Htk #Hinh]"; first done.
-    set (κ' := foldr lft_intersect static κs). wp_seq.
-    iApply ("He" $! (κ' ⊓ Λ) with "LFT Htl HE [HL Htk] HC HT").
+    set (κ' := lft_intersect_list κs). wp_seq.
+    iApply ("He" $! (κ' ⊓ Λ) with "LFT HE Htl [HL Htk] HC HT").
     rewrite /llctx_interp big_sepL_cons. iFrame "HL".
     iExists Λ. iSplit; first done. iFrame. done.
   Qed.
@@ -166,20 +163,20 @@ Section typing_rules.
     Closed [] e → UnblockTctx κ T1 T2 →
     typed_body E L C T2 e -∗ typed_body E ((κ ⊑ κs) :: L) C T1 (Endlft ;; e).
   Proof.
-    iIntros (Hc Hub) "He". iIntros (tid qE) "#LFT Htl HE".
+    iIntros (Hc Hub) "He". iIntros (tid) "#LFT #HE Htl".
     rewrite /llctx_interp big_sepL_cons. iIntros "[Hκ HL] HC HT".
     iDestruct "Hκ" as (Λ) "(% & Htok & #Hend)".
     iSpecialize ("Hend" with "Htok"). wp_bind Endlft.
     iApply (wp_mask_mono (↑lftN)); first done.
     iApply (wp_step_fupd with "Hend"). done. set_solver. wp_seq.
-    iIntros "#Hdead !>". wp_seq. iApply ("He" with "LFT Htl HE HL HC [> -]").
+    iIntros "#Hdead !>". wp_seq. iApply ("He" with "LFT HE Htl HL HC [> -]").
     iApply (Hub with "[] HT"). simpl in *. subst κ. rewrite -lft_dead_or. auto.
   Qed.
 
   Lemma type_path_instr {E L} p ty :
     typed_instruction_ty E L [p ◁ ty] p ty.
   Proof.
-    iIntros (??) "_ $$$ ?". rewrite tctx_interp_singleton.
+    iIntros (?) "_ _ $$ ?". rewrite tctx_interp_singleton.
     iApply (wp_hasty with "[-]"). done. iIntros (v) "_ Hv".
     rewrite tctx_interp_singleton. iExists v. iFrame. by rewrite eval_path_of_val.
   Qed.
@@ -195,7 +192,7 @@ Section typing_rules.
     typed_write E L ty1 ty ty1' →
     typed_instruction E L [p1 ◁ ty1; p2 ◁ ty] (p1 <- p2) (λ _, [p1 ◁ ty1']%TC).
   Proof.
-    iIntros (Hwrt tid qE) "#LFT $ HE HL".
+    iIntros (Hwrt tid) "#LFT #HE $ HL".
     rewrite tctx_interp_cons tctx_interp_singleton. iIntros "[Hp1 Hp2]".
     wp_bind p1. iApply (wp_hasty with "Hp1"). iIntros (v1) "% Hown1".
     wp_bind p2. iApply (wp_hasty with "Hp2"). iIntros (v2) "_ Hown2".
@@ -204,7 +201,7 @@ Section typing_rules.
     rewrite <-Hsz in *. destruct vl as [|v[|]]; try done.
     rewrite heap_mapsto_vec_singleton. iApply wp_fupd. wp_write.
     rewrite -heap_mapsto_vec_singleton.
-    iMod ("Hclose" with "[Hl Hown2]") as "($ & $ & Hown)".
+    iMod ("Hclose" with "[Hl Hown2]") as "($ & Hown)".
     { iExists _. iFrame. }
     rewrite tctx_interp_singleton tctx_hasty_val' //.
   Qed.
@@ -221,10 +218,10 @@ Section typing_rules.
     ty.(ty_size) = 1%nat → typed_read E L ty1 ty ty1' →
     typed_instruction E L [p ◁ ty1] (!p) (λ v, [p ◁ ty1'; v ◁ ty]%TC).
   Proof.
-    iIntros (Hsz Hread tid qE) "#LFT Htl HE HL Hp".
+    iIntros (Hsz Hread tid) "#LFT #HE Htl HL Hp".
     rewrite tctx_interp_singleton. wp_bind p. iApply (wp_hasty with "Hp").
     iIntros (v) "% Hown".
-    iMod (Hread with "[] LFT Htl HE HL Hown") as
+    iMod (Hread with "[] LFT HE Htl HL Hown") as
         (l vl q) "(% & Hl & Hown & Hclose)"; first done.
     subst v. iDestruct (ty_size_eq with "Hown") as "#>%". rewrite ->Hsz in *.
     destruct vl as [|v [|]]; try done.
@@ -243,29 +240,29 @@ Section typing_rules.
     typed_body E L C T (let: x := !p in e).
   Proof. iIntros. by iApply type_let; [apply type_deref_instr|solve_typing|]. Qed.
 
-  Lemma type_memcpy_iris E qE L qL tid ty ty1 ty1' ty2 ty2' (n : Z) p1 p2 :
+  Lemma type_memcpy_iris E L qL tid ty ty1 ty1' ty2 ty2' (n : Z) p1 p2 :
     Z.of_nat (ty.(ty_size)) = n →
     typed_write E L ty1 ty ty1' -∗ typed_read E L ty2 ty ty2' -∗
-    {{{ lft_ctx ∗ na_own tid ⊤ ∗ elctx_interp E qE ∗ llctx_interp L qL ∗
+    {{{ lft_ctx ∗ elctx_interp E ∗ na_own tid ⊤ ∗ llctx_interp L qL ∗
         tctx_elt_interp tid (p1 ◁ ty1) ∗ tctx_elt_interp tid (p2 ◁ ty2) }}}
       (p1 <-{n} !p2)
-    {{{ RET #(); na_own tid ⊤ ∗ elctx_interp E qE ∗ llctx_interp L qL ∗
+    {{{ RET #(); na_own tid ⊤ ∗ llctx_interp L qL ∗
                  tctx_elt_interp tid (p1 ◁ ty1') ∗ tctx_elt_interp tid (p2 ◁ ty2') }}}.
   Proof.
     iIntros (<-) "#Hwrt #Hread !#".
-    iIntros (Φ) "(#LFT & Htl & [HE1 HE2] & [HL1 HL2] & [Hp1 Hp2]) HΦ".
+    iIntros (Φ) "(#LFT & #HE & Htl & [HL1 HL2] & [Hp1 Hp2]) HΦ".
     wp_bind p1. iApply (wp_hasty with "Hp1"). iIntros (v1) "% Hown1".
     wp_bind p2. iApply (wp_hasty with "Hp2"). iIntros (v2) "% Hown2".
-    iMod ("Hwrt" with "[] LFT HE1 HL1 Hown1")
+    iMod ("Hwrt" with "[] LFT HE HL1 Hown1")
       as (l1 vl1) "([% %] & Hl1 & Hcl1)"; first done.
-    iMod ("Hread" with "[] LFT Htl HE2 HL2 Hown2")
+    iMod ("Hread" with "[] LFT HE Htl HL2 Hown2")
       as (l2 vl2 q2) "(% & Hl2 & Hown2 & Hcl2)"; first done.
     iDestruct (ty_size_eq with "Hown2") as "#>%". subst v1 v2. iApply wp_fupd.
     iApply (wp_memcpy with "[$Hl1 $Hl2]"); try congruence; [].
     iNext. iIntros "[Hl1 Hl2]". iApply ("HΦ" with "[> -]"). rewrite !tctx_hasty_val' //.
-    iMod ("Hcl1" with "[Hl1 Hown2]") as "($ & $ & $)".
+    iMod ("Hcl1" with "[Hl1 Hown2]") as "($ & $)".
     { iExists _. iFrame. }
-    iMod ("Hcl2" with "Hl2") as "($ & $ & $ & $)". done.
+    iMod ("Hcl2" with "Hl2") as "($ & $ & $)". done.
   Qed.
 
   Lemma type_memcpy_instr {E L} ty ty1 ty1' ty2 ty2' (n : Z) p1 p2 :
@@ -274,7 +271,7 @@ Section typing_rules.
     typed_instruction E L [p1 ◁ ty1; p2 ◁ ty2] (p1 <-{n} !p2)
                       (λ _, [p1 ◁ ty1'; p2 ◁ ty2']%TC).
   Proof.
-    iIntros (Hsz Hwrt Hread tid qE) "#LFT Htl HE HL HT".
+    iIntros (Hsz Hwrt Hread tid) "#LFT #HE Htl HL HT".
     iApply (type_memcpy_iris with "[] [] [$LFT $Htl $HE $HL HT]"); try done.
     { iApply Hwrt. }
     { iApply Hread. }
